lean/privacy/actions/info.lean
@@ -46,12 +46,12 @@ theorem RegisterInfo.events (_: RegisterInfo crypto inp m) :
   simp [register, get_events, register]
 
 --------------------
--- Create Channel --
+-- Open Channel --
 --------------------
 
-structure CreateChannelInfo (crypto: Crypto) (inp: CreateChannelInput) (m: Memory) where
+structure OpenChannelInfo (crypto: Crypto) (inp: OpenChannelInput) (m: Memory) where
   m': Memory
-  h_m': m' = (create_channel crypto inp m |> process_action crypto m).m
+  h_m': m' = (open_channel crypto inp m |> process_action crypto m).m
   j: ℕ
   h_j: j = m .ChannelsJ [inp.addrbob]
   h_Kbob: m .PublicKeys [inp.addrbob] = inp.Kbob
@@ -75,23 +75,23 @@ structure CreateChannelInfo (crypto: Crypto) (inp: CreateChannelInput) (m: Memor
   memory_diff₃: m' .OutgoingChannels [inp.outgoing_channel_id crypto, 0] = inp.r
   memory_diff₄: m' .OutgoingChannels [inp.outgoing_channel_id crypto, 1] = inp.enc_addrbob crypto
 
-def create_channel_info
-  (crypto: Crypto) (inp: CreateChannelInput) (m: Memory)
-  (success: (create_channel crypto inp m |> process_action crypto m).success = true) : CreateChannelInfo crypto inp m := by
-  let m' := (create_channel crypto inp m |> process_action crypto m).m
+def open_channel_info
+  (crypto: Crypto) (inp: OpenChannelInput) (m: Memory)
+  (success: (open_channel crypto inp m |> process_action crypto m).success = true) : OpenChannelInfo crypto inp m := by
+  let m' := (open_channel crypto inp m |> process_action crypto m).m
   let c := crypto.hash [inp.addralice, inp.kalice, inp.addrbob, inp.Kbob]
   let j := m .ChannelsJ [inp.addrbob]
 
   rw [Bool.and_eq_true] at success
   have ⟨success₀, success₁⟩ := success
-  rw [create_channel] at success₀
+  rw [open_channel] at success₀
   dsimp only [ne_eq] at success₀
   simp only [Bool.decide_and, decide_not, Bool.decide_or, Bool.and_eq_true, Bool.not_eq_eq_eq_not,
     Bool.not_true, decide_eq_false_iff_not, Bool.or_eq_true, decide_eq_true_eq] at success₀
 
   let ⟨bob_registered, alice_registered, kalice_valid, r_ne_zero, prev_outgoing_exists⟩ := success₀
 
-  simp [ServerAction.run_all, create_channel, ServerAction.run, List.foldl_cons, List.foldl_nil, write_ne] at success₁
+  simp [ServerAction.run_all, open_channel, ServerAction.run, List.foldl_cons, List.foldl_nil, write_ne] at success₁
   have ⟨⟨⟨channel_didnt_exist, h_Kbob⟩, outgoing_channel_didnt_exist⟩, _⟩ := success₁
 
   exact {
@@ -109,25 +109,25 @@ def create_channel_info
     outgoing_channel_didnt_exist := outgoing_channel_didnt_exist,
     no_change := by
       intro t x ⟨h₀, h₁, h₂, h₃, h₄⟩
-      simp [m', h₂, h₃, h₄, create_channel, ServerAction.run_all, ServerAction.run]
+      simp [m', h₂, h₃, h₄, open_channel, ServerAction.run_all, ServerAction.run]
       rw [write_ne h₁]
       simp [h₀]
-    memory_diff₀ := by simp [m', create_channel, ServerAction.run_all, ServerAction.run]
+    memory_diff₀ := by simp [m', open_channel, ServerAction.run_all, ServerAction.run]
     memory_diff₁ := by
-      simp [m', create_channel, ServerAction.run_all, ServerAction.run]
+      simp [m', open_channel, ServerAction.run_all, ServerAction.run]
       rw [write_eq]
-    memory_diff₂ := by simp [m', create_channel, ServerAction.run_all, ServerAction.run]
-    memory_diff₃ := by simp [m', create_channel, ServerAction.run_all, ServerAction.run]
-    memory_diff₄ := by simp [m', create_channel, ServerAction.run_all, ServerAction.run]
+    memory_diff₂ := by simp [m', open_channel, ServerAction.run_all, ServerAction.run]
+    memory_diff₃ := by simp [m', open_channel, ServerAction.run_all, ServerAction.run]
+    memory_diff₄ := by simp [m', open_channel, ServerAction.run_all, ServerAction.run]
   }
 
 -----------------------
--- Create Subchannel --
+-- Open Subchannel --
 -----------------------
 
-structure CreateSubchannelInfo (crypto: Crypto) (inp: CreateSubchannelInput) (m: Memory) where
+structure OpenSubchannelInfo (crypto: Crypto) (inp: OpenSubchannelInput) (m: Memory) where
   m': Memory
-  h_m': m' = (create_subchannel crypto inp m |> process_action crypto m).m
+  h_m': m' = (open_subchannel crypto inp m |> process_action crypto m).m
   r_ne_zero: inp.r ≠ 0
   channel_exists: m .ChannelHashes [crypto.hash [inp.c, inp.addralice, inp.addrbob, inp.Kbob]] ≠ 0
   prev_subchannel_exists: inp.k₁ = 0 ∨ m .SubchannelTokens [crypto.hash [inp.c, inp.k₀, inp.k₁ - 1], 0] ≠ 0
@@ -143,13 +143,13 @@ structure CreateSubchannelInfo (crypto: Crypto) (inp: CreateSubchannelInput) (m:
   memory_diff₁: m' .SubchannelTokens [inp.subchannel_id crypto, 1] = inp.enc crypto
   memory_diff₂: m' .SubchannelHashes [inp.subchannel_hash crypto] = 1
 
-def create_subchannel_info
-  (crypto: Crypto) (inp: CreateSubchannelInput) (m: Memory)
-  (success: (create_subchannel crypto inp m |> process_action crypto m).success = true)
-  : CreateSubchannelInfo crypto inp m := by
-  let m' := (create_subchannel crypto inp m |> process_action crypto m).m
+def open_subchannel_info
+  (crypto: Crypto) (inp: OpenSubchannelInput) (m: Memory)
+  (success: (open_subchannel crypto inp m |> process_action crypto m).success = true)
+  : OpenSubchannelInfo crypto inp m := by
+  let m' := (open_subchannel crypto inp m |> process_action crypto m).m
 
-  unfold create_subchannel at success
+  unfold open_subchannel at success
   simp only [Bool.and_eq_true] at success
   have ⟨success₀, success₁⟩ := success
   simp only [ne_eq, bne_iff_ne, Bool.decide_and, decide_not, Bool.decide_or,
@@ -173,10 +173,10 @@ def create_subchannel_info
     k₀_lt_MAX_K₀ := k₀_lt_MAX_K₀,
     no_change := by
       intro t x h₀ h₁ h₂
-      simp [m', h₀, h₁, h₂, create_subchannel, ServerAction.run_all, ServerAction.run]
-    memory_diff₀ := by simp [m', create_subchannel, ServerAction.run_all, ServerAction.run]
-    memory_diff₁ := by simp [m', create_subchannel, ServerAction.run_all, ServerAction.run]
-    memory_diff₂ := by simp [m', create_subchannel, ServerAction.run_all, ServerAction.run]
+      simp [m', h₀, h₁, h₂, open_subchannel, ServerAction.run_all, ServerAction.run]
+    memory_diff₀ := by simp [m', open_subchannel, ServerAction.run_all, ServerAction.run]
+    memory_diff₁ := by simp [m', open_subchannel, ServerAction.run_all, ServerAction.run]
+    memory_diff₂ := by simp [m', open_subchannel, ServerAction.run_all, ServerAction.run]
   }
 
 -----------------
