lean/privacy/transactions/immutability.lean
@@ -44,8 +44,8 @@ theorem immutability₀ (crypto: Crypto) (m: Memory) (action: Action) (t: Memory
       exact h_nonzero info.alice_was_not_registered
     )]
 
-  case CreateChannel inp =>
-    let info := create_channel_info crypto inp m success
+  case OpenChannel inp =>
+    let info := open_channel_info crypto inp m success
     rw [run_action, ←info.h_m', info.no_change _ _ (by
       simp only [ne_eq, Prod.mk.injEq, h_t, false_and, not_false_eq_true, not_and, true_and]
       refine ⟨?_, ?_, ?_⟩
@@ -59,8 +59,8 @@ theorem immutability₀ (crypto: Crypto) (m: Memory) (action: Action) (t: Memory
       · intro h₀ h₁; simp [h₀, h₁] at h_t
     )]
 
-  case CreateSubchannel inp =>
-    let info := create_subchannel_info crypto inp m success
+  case OpenSubchannel inp =>
+    let info := open_subchannel_info crypto inp m success
     rw [run_action, ←info.h_m', info.no_change _ _
       (λ h' ↦ h_nonzero (by rw [Prod.mk.injEq] at h'; simp [h'.1, h'.2, info.old_hash_was_zero]))
       (λ h' ↦ h_nonzero (by rw [Prod.mk.injEq] at h'; simp [h'.1, h'.2, info.old_token_was_zero]))
@@ -190,13 +190,13 @@ theorem immutable_fn_prop {m₀ m₁: Memory} {f: Functional Bool} (imm: immutab
   intro h
   rw [imm (by simp [h])]
 
-theorem create_channel_immutable
-    {crypto: Crypto} {m₀ m₁: Memory} (inp: CreateChannelInput)
+theorem open_channel_immutable
+    {crypto: Crypto} {m₀ m₁: Memory} (inp: OpenChannelInput)
     (imm₀: ∀ x, immutable_fn m₀ m₁ (mem_cell_fn .PublicKeys x))
     (imm₁: ∀ x, immutable_fn m₀ m₁ (mem_cell_fn .OutgoingChannels [x, 0]))
-    (success: (run_action₀ crypto (.CreateChannel inp) m₀).2) :
-    run_action₀ crypto (.CreateChannel inp) m₁ = run_action₀ crypto (.CreateChannel inp) m₀ := by
-  dsimp only [run_action₀, create_channel] at *
+    (success: (run_action₀ crypto (.OpenChannel inp) m₀).2) :
+    run_action₀ crypto (.OpenChannel inp) m₁ = run_action₀ crypto (.OpenChannel inp) m₀ := by
+  dsimp only [run_action₀, open_channel] at *
   rw [decide_eq_true_iff] at success
 
   have ⟨h₀, h₁, h₂, h₃, h₄⟩ := success
@@ -213,13 +213,13 @@ theorem create_channel_immutable
     case inl h₄ => simp [h₄]
     case inr h₄ => rw [imm₁ _ h₄]
 
-theorem create_subchannel_immutable
-    {crypto: Crypto} {m₀ m₁: Memory} (inp: CreateSubchannelInput)
+theorem open_subchannel_immutable
+    {crypto: Crypto} {m₀ m₁: Memory} (inp: OpenSubchannelInput)
     (imm₀: ∀ x, immutable_fn m₀ m₁ (mem_cell_fn .ChannelHashes x))
     (imm₁: ∀ x, immutable_fn m₀ m₁ (mem_cell_fn .SubchannelTokens [x, 0]))
-    (success: (run_action₀ crypto (.CreateSubchannel inp) m₀).2) :
-    run_action₀ crypto (.CreateSubchannel inp) m₁ = run_action₀ crypto (.CreateSubchannel inp) m₀ := by
-  dsimp only [run_action₀, create_subchannel] at *
+    (success: (run_action₀ crypto (.OpenSubchannel inp) m₀).2) :
+    run_action₀ crypto (.OpenSubchannel inp) m₁ = run_action₀ crypto (.OpenSubchannel inp) m₀ := by
+  dsimp only [run_action₀, open_subchannel] at *
   rw [decide_eq_true_iff] at success
   have ⟨h₀, h₁, h₂, h₃⟩ := success
 
@@ -313,8 +313,8 @@ theorem run_action₀_immutable
     run_action₀ crypto actions m₁ = run_action₀ crypto actions m₀ := by
   cases actions
   case Register inp => trivial
-  case CreateChannel inp => exact create_channel_immutable inp imm.imm₃ imm.imm₄ success
-  case CreateSubchannel inp => exact create_subchannel_immutable inp imm.imm₀ imm.imm₁ success
+  case OpenChannel inp => exact open_channel_immutable inp imm.imm₃ imm.imm₄ success
+  case OpenSubchannel inp => exact open_subchannel_immutable inp imm.imm₀ imm.imm₁ success
   case CreateNote inp => exact create_note_immutable inp imm.imm₂ imm.imm₅ success
   case CancelNote inp => exact cancel_note_immutable inp imm.imm₂ imm.imm₆ success
   case OpenDeposit inp => trivial
